updated sample and deleted extraneous samples

Test/civl/tds.bpl
@@ -1,19 +1,11 @@
+// RUN: %boogie -noinfer -typeEncoding:m -useArrayTheory "%s" > "%t"
+// RUN: %diff "%s.expect" "%t"
+
 function {:builtin "MapConst"} MapConstBool(bool): [int]bool;
 function {:inline} {:linear "tid"} TidCollector(x: int) : [int]bool
 {
   MapConstBool(false)[x := true]
 }
-
-type{:datatype} Pid;
-function{:constructor} Client(id:int):Pid;
-function{:constructor} Server(id:int):Pid;
-function{:constructor} Master(id:int):Pid;
-
-type{:datatype} Msg;
-function{:constructor} Request(cid:int):Msg;
-function{:constructor} None():Msg;
-function{:constructor} Task():Msg;
-function{:constructor} Ack(cid:int):Msg;
 
 const unique DEFAULT: int;
 const unique CREATED: int;
@@ -22,186 +14,123 @@ const unique FINISHED: int;
 
 var status:[int]int;
 
-procedure {:atomic}  {:layer 5} atomic_main({:linear "tid"} id: int, n: int)
+procedure {:atomic} {:layer 5} atomic_main({:linear "tid"} id: int, {:linear_in "tid"} tids: [int]bool)
 modifies status;
 {
-    var newStatus:[int]int;
     assert id == c;
+    assert (forall i: int :: (0 <= i && i < n) <==> tids[i]);    
     assert (forall i: int :: 0 <= i && i < n ==> status[i] == DEFAULT);
-    assume (forall i: int :: 0 <= i && i < n ==> newStatus[i] == FINISHED);
-    assume (forall i: int :: (0 <= i && i < n) || newStatus[i] == status[i]);    
-    status := newStatus;
-//    status := (lambda j: int :: if (0 <= j && j < n) then FINISHED else status[j]);
+    status := (lambda j: int :: if (0 <= j && j < n) then FINISHED else status[j]);
 }
 
-procedure {:left}  {:layer 4} atomic_server({:linear "tid"} id: int, sid: int, n: int)
+procedure {:left} {:layer 4} atomic_server({:linear "tid"} id: int, {:linear_in "tid"} tids: [int]bool)
 modifies status;
 {
-    var newStatus:[int]int;
     assert id == c;
+    assert (forall i: int :: (0 <= i && i < n) <==> tids[i]);
     assert (forall i: int :: 0 <= i && i < n ==> status[i] == DEFAULT);
-    assume (forall i: int :: 0 <= i && i < n ==> newStatus[i] == CREATED);
-    assume (forall i: int :: (0 <= i && i < n) || newStatus[i] == status[i]);
-    status := newStatus;
-//    status := (lambda j: int :: if (0 <= j && j < n) then CREATED else status[j]);
+    status := (lambda j: int :: if (0 <= j && j < n) then CREATED else status[j]);
 }
 
-procedure {:left}  {:layer 4} atomic_client({:linear "tid"} id: int, sid: int, mid: int, n: int)
+procedure {:left} {:layer 4} atomic_client({:linear "tid"} id: int)
 modifies status;
 {
-    var newStatus:[int]int;
     assert id == c;
     assert (forall i: int :: 0 <= i && i < n ==> status[i] == CREATED);
-    assume (forall i: int :: 0 <= i && i < n ==> newStatus[i] == PROCESSED);
-    assume (forall i: int :: (0 <= i && i < n) || newStatus[i] == status[i]);
-    status := newStatus;
-//    status := (lambda j: int :: if (0 <= j && j < n) then PROCESSED else status[j]);
+    status := (lambda j: int :: if (0 <= j && j < n) then PROCESSED else status[j]);
 }
 
-procedure {:left}  {:layer 4} atomic_master({:linear "tid"} id: int, mid: int, n: int)
+procedure {:left} {:layer 4} atomic_master({:linear "tid"} id: int)
 modifies status;
 {
-    var newStatus:[int]int;
     assert id == c;
     assert (forall i: int :: 0 <= i && i < n ==> status[i] == PROCESSED);
-    assume (forall i: int :: 0 <= i && i < n ==> newStatus[i] == FINISHED);
-    assume (forall i: int :: (0 <= i && i < n) || newStatus[i] == status[i]);
-    status := newStatus;
-//    status := (lambda j: int :: if (0 <= j && j < n) then FINISHED else status[j]);
+    status := (lambda j: int :: if (0 <= j && j < n) then FINISHED else status[j]);
 }
 
 const c: int;
+const n: int;
+axiom 0 <= n;
 
-procedure {:yields} {:layer 4} {:refines "atomic_main"} main({:linear "tid"} id: int, n: int)
+procedure {:yields} {:layer 4} {:refines "atomic_main"} main({:linear "tid"} id: int, {:linear_in "tid"} tids: [int]bool)
 {
     var i: int;
-    var m: Msg;
     var sid: int;
     var mid: int;
     var cid: int;
 
     yield;
-    call server3(id, 0, n);
-    call client3(id, 0, 0, n);
-    call master3(id, 0, n);
+    call server3(id, tids);
+    call client3(id);
+    call master3(id);
     yield;
 }
 
-procedure {:yields} {:layer 3} {:refines "atomic_server"} server3({:linear "tid"} id: int, sid: int, n: int)
+procedure {:layer 3} StatusSnapshot() returns (snapshot: [int]int);
+ensures snapshot == status;
+
+procedure {:yields} {:layer 2} {:refines "AtomicAlloc"} Alloc(i: int, {:linear_in "tid"} tidq: [int]bool) returns ({:linear "tid"} id: int, {:linear "tid"} tidq':[int]bool);
+procedure {:both} {:layer 3} AtomicAlloc(i: int, {:linear_in "tid"} tidq: [int]bool) returns ({:linear "tid"} id: int, {:linear "tid"} tidq':[int]bool)
+{ assert tidq[i]; id := i; tidq' := tidq[i := false]; }
+
+procedure {:yields} {:layer 3} {:refines "atomic_server"} server3({:linear "tid"} id: int, {:linear_in "tid"} tids: [int]bool)
 {
     var i: int;
+    var {:layer 3} snapshot: [int]int;
+    var {:linear "tid"} tids': [int]bool;
+    var {:linear "tid"} tid: int;
     yield;
     i := 0;
+    call snapshot := StatusSnapshot();
+    tids' := tids;
     while (i < n)
     invariant {:terminates} {:layer 2,3} true;
+    invariant {:layer 3} 0 <= i && i <= n;
+    invariant {:layer 3} (forall j: int :: i <= j && j < n <==> tids'[j]);
+    invariant {:layer 3} status == (lambda j: int :: if (0 <= j && j < i) then CREATED else snapshot[j]);
     {
-        async call server2(sid, i);
+        call tid, tids' := Alloc(i, tids');
+        async call server2(tid);
         i := i + 1;
     }
     yield;
 }
 
-procedure {:left} {:layer 3} atomic_server2(sid: int, i: int)
+procedure {:left} {:layer 3} atomic_server2({:linear "tid"} i: int)
 modifies status;
 {
     assert status[i] == DEFAULT;
     status[i] := CREATED;
 }
-procedure {:yields} {:layer 2} {:refines "atomic_server2"} server2(sid: int, i: int);
+procedure {:yields} {:layer 2} {:refines "atomic_server2"} server2({:linear "tid"} i: int);
 
-procedure {:yields} {:layer 3} {:refines "atomic_client"} client3({:linear "tid"} id: int, sid: int, mid: int, n: int)
+procedure {:yields} {:layer 3} {:refines "atomic_client"} client3({:linear "tid"} id: int)
 {
     yield;
-    call client2(sid, mid, n);
+    call client2();
     yield;
 }
 
-procedure {:atomic} {:layer 3} atomic_client2(sid: int, mid: int, n: int)
+procedure {:atomic} {:layer 3} atomic_client2()
 modifies status;
 {
-    var newStatus:[int]int;
-    assert (forall i: int :: 0 <= i && i < n ==> status[i] == CREATED);
-    assume (forall i: int :: 0 <= i && i < n ==> newStatus[i] == PROCESSED);
-    assume (forall i: int :: (0 <= i && i < n) || newStatus[i] == status[i]);
-    status := newStatus;
+    assume (forall i: int :: 0 <= i && i < n ==> status[i] == CREATED);
+    status := (lambda j: int :: if (0 <= j && j < n) then PROCESSED else status[j]);
 }
-procedure {:yields} {:layer 2} {:refines "atomic_client2"} client2(sid: int, mid: int, n: int);
+procedure {:yields} {:layer 2} {:refines "atomic_client2"} client2();
 
-procedure {:yields} {:layer 3} {:refines "atomic_master"} master3({:linear "tid"} id: int, mid: int, n: int)
+procedure {:yields} {:layer 3} {:refines "atomic_master"} master3({:linear "tid"} id: int)
 {
     yield;
-    call master2(mid, n);
+    call master2();
     yield;
 }
 
-procedure {:atomic} {:layer 3} atomic_master2(mid: int, n: int)
+procedure {:atomic} {:layer 3} atomic_master2()
 modifies status;
 {
-    var newStatus:[int]int;
     assert (forall i: int :: 0 <= i && i < n ==> status[i] == PROCESSED);
-    assume (forall i: int :: 0 <= i && i < n ==> newStatus[i] == FINISHED);
-    assume (forall i: int :: (0 <= i && i < n) || newStatus[i] == status[i]);
-    status := newStatus;
+    status := (lambda j: int :: if (0 <= j && j < n) then FINISHED else status[j]);    
 }
-procedure {:yields} {:layer 2} {:refines "atomic_master2"} master2(mid: int, n: int);
+procedure {:yields} {:layer 2} {:refines "atomic_master2"} master2();
 
-/*
-procedure {:inline} CreateTask(cid: int)
-{
-    assert status[cid] == DEFAULT;
-    status[cid] := CREATED;
-}
-
-procedure {:inline} ProcessTask(cid: int)
-{
-    assert status[cid] == CREATED;
-    status[cid] := PROCESSED;
-}
-
-procedure {:inline} FinishTask(cid: int)
-{
-    assert status[cid] == PROCESSED;
-    status[cid] := FINISHED;
-}
-
-procedure Send(id: int, m: Msg);
-procedure ServerReceive(sid: int) returns (m: Msg);
-procedure ClientReceive(cid: int) returns (m: Msg);
-procedure MasterReceive(mid: int) returns (m: Msg);
-
-procedure server(sid: int, n: int)
-{
-    var i: int;
-    var m: Msg;
-    i := 0;
-    while (i < n) {
-        call m := ServerReceive(sid);
-	assert is#Request(m);
-	call CreateTask(cid#Request(m)); // DEFAULT -> CREATED	
-	call Send(cid#Request(m), Task());
-	i := i + 1;
-    }
-}
-
-procedure client(cid: int, sid: int, mid: int)
-{
-    var m: Msg;
-    call Send(sid, Request(cid));
-    call m := ClientReceive(cid);
-    assert is#Task(m);
-    call ProcessTask(cid); // CREATED -> PROCESSED
-    call Send(mid, Ack(cid));
-}
-
-procedure master(mid: int, n: int) {
-    var m: Msg;
-    var i: int;
-    i := 0;
-    while (i < n) { 
-        call m := MasterReceive(mid);
-	assert is#Ack(m);
-	call FinishTask(cid#Ack(m)); // PROCESSED -> FINISHED
-	i := i + 1;
-    }
-}
-*/
